🚧 Draft new, flatter type system

theories/autosubst/AST.sig
@@ -1,10 +1,10 @@
 list : Functor
+option : Functor
 
 -- Global references
 gref : Type
 
--- Extension references
-eref : Type
+-- Assumption references
 aref : Type
 
 -- Universe levels
@@ -20,5 +20,5 @@ Pi : term -> (bind term in term) -> term
 lam : term -> (bind term in term) -> term
 app : term -> term -> term
 
-const : gref -> "list" ("list" (term)) -> term
-assm : eref -> aref -> term
+const : gref -> "list" ("option" (term)) -> term
+assm : aref -> term
