theories/BasicAST.v
@@ -2,14 +2,11 @@ From Stdlib Require Import Utf8 String.
 
 Set Primitive Projections.
 
-(** Reference in the global environment **)
+(** Reference in the global environment *)
 Definition gref := string.
 
-(** Reference in the extension environment (de Bruijn level) **)
-Definition eref := nat.
-
-(** Reference in an extension instance (de Bruijn index) **)
+(** Reference to an assumption (de Bruijn level) *)
 Definition aref := nat.
 
-(** Universe level **)
+(** Universe level *)
 Definition level := nat.
